%!LW recipe=latexmk
\documentclass[11pt,a4paper]{article}
\input\input{../macros.tex}
\title{Learning Notes}
\author{Yingjie Zhu}
\date{\today}


\begin{document}
\maketitle

\section{Theory of Real Variable Function}

\begin{exercise}
    let $f: \Omega \to \mathbb{R}$ be simple non-negative measurable function. And $E_k \subseteq \Omega $ be a sequence of increasing
    measurable sets. 
    And let

    \[
        E = \bigcup_{k=1}^{\infty}E_k
    \]

    then we have

    \[
        \int_{E}f(x) \mathrm{d}x = \lim_{k \to \infty}\int_{E_k}f(x) \mathrm{d}x
    \]

\end{exercise}

\begin{proof}
    since $f$ is simple non-negative measurable function on $\Omega$, and $E_k$ is measurable. So $f$ is also a simple non-negative measurable function on $E_k$.

    let 

    \[
        f(x) = \sum_{i=1}^{N}c_i \chi_{F_i}\quad x \in \Omega
    \]

    then $f(x)$ also be


    \[
        f(x) = \sum_{i=1}^{N}c_i \chi_{F_i \cap E_k}\quad x \in E_k
    \]

    so we have

    \[
        \int_{E_k} f(x) \mathrm{d}x = \sum_{i=1}^{N}c_i m(F_i \cap E_k)
    \]

    and 


    \[
        \lim_{k \to \infty}\int_{E_k} f(x) \mathrm{d}x = \sum_{i=1}^{N}c_i \lim_{k \to \infty}m(F_i \cap E_k)
    \]

    since $F_i \cap E_k$ is increasing and measurable, so we have

    \[
        \lim_{k \to \infty}m(F_i \cap E_k) = m(\lim_{k \to \infty}\left( F_i \cap E_k \right)) = m(F_i \cap E)
    \]

    so 

    \begin{align*}
        \lim_{k \to \infty}\int_{E_k} f(x) \mathrm{d}x &= \sum_{i=1}^{N}c_i \lim_{k \to \infty}m(F_i \cap E_k) \\
        &= \sum_{i=1}^{N}c_i m(F_i \cap E) = \int_{E}f(x) \mathrm{d}x
    \end{align*}
\end{proof}

\begin{exercise}
    let $f_n: \Omega \to \mathbb{R}^*$ be increasing non-negative measurable functions. and $f_n \to f$ point wise.
    then we have 

    \[
        \lim_{n \to \infty}\int_{\Omega}f_n(x) \mathrm{d}x = \int_{\Omega}f(x) \mathrm{d}x
    \]
\end{exercise}

\begin{proof}
    since $f_n$ is measurable and $f_n \to f$, so $f$ is also measurable. and $f$ is non-negative. So

    \[
        \int_{\Omega}f(x) \mathrm{d}x
    \]

    is well defined.

    since $f_k \le f$, so we have

    \[
        \int_{\Omega}f_k(x) \mathrm{d}x \le \int_{\Omega}f(x) \mathrm{d}x
    \]

    take $k \to \infty$, we have

    \[
        \lim_{k \to \infty}\int_{\Omega}f_k(x) \mathrm{d}x \le \int_{\Omega}f(x) \mathrm{d}x
    \]

    consider a simple non-negative function $h: \Omega \to \mathbb{R}$, and $h(x) \le f(x)$, take any $c \in (0,1)$, we have

    \[
        \lim_{k \to \infty}f_k(x) = f(x) \ge ch(x)
    \]

    let 

    \[
        E_k = \{x: f_k(x) \ge ch(x) \}
    \]

    we have increasing sets $E_k$ and

    \[
        \Omega = \bigcup_{k=1}^{\infty}E_k
    \]

    so we have

    \[
    \int_{E_k}ch(x)\mathrm{d}x \le \int_{E_k}f_k(x) \mathrm{d}x \le \int_{\Omega}f_k(x) \mathrm{d}x
    \]

    take $k \to \infty$, we have

    \[
    \lim_{k \to \infty}\int_{\Omega}f_k(x) \mathrm{d}x \ge c \int_{\Omega}h(x) \mathrm{d}x
    \]

    take $c \to 1$, we have


    \[
    \lim_{k \to \infty}\int_{\Omega}f_k(x) \mathrm{d}x \ge  \int_{\Omega}h(x) \mathrm{d}x
    \]

    by definition of integral on non-negative measurable function take

    \[
        \int_{\Omega}h(x) \mathrm{d}x \to \int_{\Omega}f(x) \mathrm{d}x
    \]

    then we have

    \[
    \lim_{k \to \infty}\int_{\Omega}f_k(x) \mathrm{d}x \ge  \int_{\Omega}f(x) \mathrm{d}x
    \]
\end{proof}

\begin{exercise}
    let $f: \Omega \to \mathbb{R}^*$ and $g: \Omega \to \mathbb{R}^*$ be non-negative measurable function, then we have

    \[
        \int_{\Omega}f(x) + g(x) \mathrm{d}x = \int_{\Omega}f(x) \mathrm{d}x + \int_{\Omega} g(x) \mathrm{d}x
    \]
\end{exercise}

\begin{proof}
    since $f: \Omega \to \mathbb{R}^*$ is non-negative measurable function, then there exists a sequence of 
    simple non-negative function $f_n: \Omega \to \mathbb{R}$ and $f_n \to f$ point wise. Also for $g$ and $g_n$
    by law of limits we have $f_n + g_n \to f + g$ point wise, and $f_n + g_n$ be increasing

    then we have

    \begin{align*}
        \int_{\Omega}f(x) \mathrm{d}x + \int_{\Omega} g(x) \mathrm{d}x &= \lim_{n \to \infty}\int_{\Omega}f_n \mathrm{d}x + \lim_{n \to \infty}\int_{\Omega}g_n \mathrm{d}x \\
        &= \lim_{n \to \infty}\left( \int_{\Omega}f_n(x) \mathrm{d}x + \int_{\Omega}g_n(x) \mathrm{d}x\right) \\
        &= \lim_{n \to \infty}\left( \int_{\Omega} \left( f_n+g_n \right) \mathrm{d}x \right) \\
        &= \int_{\Omega} \left( f + g \right) \mathrm{d}x
    \end{align*}
\end{proof}

\begin{exercise}
    let $f_n: \Omega \to \mathbb{R}$ be decreasing non-negative measurable function sequence. And $f_n \to f$ point wise.
    then we have

    \[
        \lim_{n \to \infty}\int_{\Omega}f_n \mathrm{d}x = \int_{\Omega}f \mathrm{d}x
    \]

\end{exercise}

\begin{proof}
    since $f_1, f_2, .. $ is decreasing. let $g_1 = f_1, g_2 = f_1 - f_2, ..$. then $g_n$ is increasing and non-negative. and $g_n \to f_1 - f$ point wise

    so we have

    \[
        \lim_{n \to \infty}\int_{\Omega}g_n \mathrm{d}x = \int_{\Omega}f_1 - f \mathrm{d}x
    \]


    add items to both side:

    \begin{align*}
        \lim_{n \to \infty}\int_{\Omega}g_n \mathrm{d}x + \int_{\Omega}f \mathrm{d}x &= \int_{\Omega}f_1 - f \mathrm{d}x + \int_{\Omega}f \mathrm{d}x \\
        \lim_{n \to \infty}\int_{\Omega}g_n \mathrm{d}x + \int_{\Omega}f \mathrm{d}x &= \int_{\Omega}f_1 \mathrm{d}x \\
        \lim_{n \to \infty}\int_{\Omega}f_n \mathrm{d}x + \lim_{n \to \infty}\int_{\Omega}g_n \mathrm{d}x + \int_{\Omega}f \mathrm{d}x &= \int_{\Omega}f_1 \mathrm{d}x + \lim_{n \to \infty}\int_{\Omega}f_n \mathrm{d}x\\
        \lim_{n \to \infty}\int_{\Omega}\left(f_n + g_n\right) \mathrm{d}x  + \int_{\Omega}f \mathrm{d}x &= \int_{\Omega}f_1 \mathrm{d}x + \lim_{n \to \infty}\int_{\Omega}f_n \mathrm{d}x\\ 
        \int_{\Omega}f_1 \mathrm{d}x + \int_{\Omega}f \mathrm{d}x &= \int_{\Omega}f_1 \mathrm{d}x + \lim_{n \to \infty}\int_{\Omega}f_n \mathrm{d}x \\
        \int_{\Omega}f \mathrm{d}x &= \lim_{n \to \infty}\int_{\Omega}f_n \mathrm{d}x \\
    \end{align*}
\end{proof}

\begin{exercise}
    let $f: \Omega \to \mathbb{R}$ be simple non-negative measurable function. And $E \subseteq \Omega$. Then we have

    \[
        \int_{E} f \mathrm{d}x = \int_{\Omega} f(x)\chi_{E}(x) \mathrm{d}x
    \]
\end{exercise}

\begin{proof}
   let 
   
   \[
    f(x) = \sum_{i=1}^{N}c_i \chi_{F_i}(x) \quad x \in \Omega
   \]


   then we have

   \begin{align*}
    \int_{E}f \mathrm{d}x &= \sum_{i=1}^{N} c_i m(F_i \cap E) \\
   \end{align*}

   and $f \chi_{E}$ is simple non-negative measurable function on $E \cap F_1, E \cap F_2, .., \Omega \setminus E$

   \begin{align*}
    \int_{\Omega}f \chi_{E} \mathrm{d}x  = \sum_{i=1}^{N} c_i m(E \cap F_i) + 0
   \end{align*}
\end{proof}


\begin{exercise}
    let non-negative measurable function $f: \Omega \to \mathbb{R}^*$ and $g \to \mathbb{R}^*$ meets 

    \[
        f(x) = g(x)\quad \text{a.e.}
    \]

    prove that

    \[
        \int_{\Omega}f \mathrm{d}x = \int_{\Omega}g \mathrm{d}x
    \]

    let 

    \[
        E = \{ x \in \Omega : f(x) = g(x) \}
    \]

    and $E' = \Omega \setminus E$

    then we have

    \begin{align*}
        \int_{\Omega}f \mathrm{d}x &= \int_{\Omega}f(\chi_{E} + \chi_{E'}) \mathrm{d}x \\
        &= \int_{E}f \mathrm{d}x  + \int_{E'}f\mathrm{d}x \\
        &= \int_{E}g \mathrm{d}x  + \int_{E'}f\mathrm{d}x \\
        &= \int_{E}g \mathrm{d}x  + 0 \\
        &= \int_{E}g \mathrm{d}x  + \int_{E'}g\mathrm{d}x \\
        &= \int_{\Omega}g \mathrm{d}x
    \end{align*}
\end{exercise}

\begin{thm}[Fatou's Theorem]
    let $f_n: \Omega \to \mathbb{R}^*$ be sequence of non-negative measurable functions. Then

    \[
        \int_{\Omega} \left(\varliminf_{n \to \infty} f_n \right) \mathrm{d}x \le \varliminf_{n \to \infty} \int_{\Omega} f_n \mathrm{d}x
    \]
\end{thm}

\begin{proof}
    let 

    \[
        h_n(x) = \inf_{m \ge n}f_m(x)
    \]

    then we have

    \[
        \varliminf_{n \to \infty}f_n = \lim_{n \to \infty} h_n
    \]

    and

    \[  
        h_n \le h_{n+1}
    \]

    by Beppo levi's theorem we have

    \[
\int_{\Omega} \left(\varliminf_{n \to \infty} f_n \right) \mathrm{d}x = \lim_{n \to \infty} \int_{\Omega}h_n \mathrm{d}x
    \]

    since we have

    \[
        h_n \le f_n
    \]

    so we have

    \[
\int_{\Omega} \left(\varliminf_{n \to \infty} f_n \right) \mathrm{d}x = \lim_{n \to \infty} \int_{\Omega}h_n \mathrm{d}x \le \lim_{n \to \infty} \int_{\Omega}f_n \mathrm{d}x
    \]
\end{proof}

\end{document}














