%!LW recipe=latexmk
\documentclass[11pt,a4paper]{article}
\input\input{../macros.tex}
\title{Learning Notes}
\author{Yingjie Zhu}
\date{\today}


\begin{document}
\maketitle

\section{Theory of Real Variable Function}

\begin{exercise}
    if $f_n$ is measurable, then 

    \[
        f(x) = \sup_{n=1}^{\infty}f_n(x)
    \]

    is also measurable
\end{exercise}

\begin{proof}
   we have 
   
   \begin{align*}
        \bigcup_{n=1}^{\infty}(-\infty, a_n) = (-\infty, \sup_{n=1}^{\infty}a_n)
   \end{align*}

   so 

   \[
    \{ x \vert f(x) > t \} = \bigcup_{n=1}^{\infty} \{ x \vert f_n(x) >  t\}
   \]
\end{proof}

\begin{exercise}
    if $f_n$ is measurable, then 

    \[
        f(x) = \inf_{n=1}^{\infty}f_n(x)
    \]

    is also measurable
\end{exercise}

\begin{proof}
    
\begin{align*}
    & \bigcup_{j=1}^{\infty}\bigcap_{n=1}^{\infty}\bigcap_{k=1}^{\infty}(-\infty, a_n + \frac{1}{k} - \frac{1}{j}) = \bigcup_{j=1}^{\infty}\bigcap_{n=1}^{\infty}(-\infty, a_n  - \frac{1}{j}] \\
    & = \bigcup_{j=1}^{\infty}(-\infty, \left( \inf_{n=1}^{\infty}a_n \right)  - \frac{1}{j}] \\
    & = (-\infty, \left( \inf_{n=1}^{\infty}a_n \right))
\end{align*}

so we have

\[
    \{ x \vert f(x) > t \} = \bigcup_{j=1}^{\infty}\bigcap_{n=1}^{\infty}\bigcap_{k=1}^{\infty} \{ f_n(x) + \frac{1}{k} - \frac{1}{j} > t \}
\]

\end{proof}


\begin{exercise}
    if $f_n$ is measurable, then 

    \[
        f(x) = \varlimsup_{n \to \infty}f_n(x)
    \]

    is also measurable
\end{exercise}

\begin{proof}
    
    \[
        f(x) = \inf_{n=1}^{\infty} \left( \sup_{m=n}^{\infty} f_m(x) \right)
    \]

    since

    \[
        h_n = \left( \sup_{m=n}^{\infty} f_m(x) \right)
    \]

    is measurable, so

    \[
        f(x) = \inf_{n=1}^{\infty} h_n(x)
    \]

    is measurable
\end{proof}

\begin{exercise}
    prove that:
    \[
        \inf_{n=1}^{\infty} a_n = - \sup_{n=1}^{\infty}-a_n
    \]
\end{exercise}

\begin{proof}
    part 1:
    \begin{align*}
        \inf_{n=1}^{\infty} a_n &\le a_n \\
        -a_n & \le -\inf_{n=1}^{\infty} a_n \\
        \sup_{n=1}^{\infty} - a_n & \le -\inf_{n=1}^{\infty} a_n \\
        \inf_{n=1}^{\infty} a_n & \le -\sup_{n=1}^{\infty} - a_n\\
    \end{align*}

    part 2:

    \begin{align*}
        -a_n &\le \sup_{n=1}^{\infty}-a_n \\
-\sup_{n=1}^{\infty}-a_n & \le a_n \\
-\sup_{n=1}^{\infty}-a_n & \le \inf_{n=1}^{\infty}a_n \\
    \end{align*}
\end{proof}

\begin{exercise}
    let $f$ be measurable, prove that $h(x) = \max (f(x), 0)$ is also measurable.
\end{exercise}

\begin{proof}
    \[
        \{ x \vert h(x) > t \}  = \{ x \vert f(x) > t \} \cup \{ x \vert 0 > t \}
    \]
\end{proof}


\begin{exercise}
    let $f$ be measurable, prove that $h(x) = \min (f(x), 0)$ is also measurable.
\end{exercise}

\begin{proof}
    \[
        \min(f(x), 0) = - \max(-f(x), 0)
    \]
\end{proof}


\begin{exercise}
    let $f$ be measurable, prove that $h(x) = \lvert f(x)\rvert$ is also measurable.
\end{exercise}

\begin{proof}
    \[
\lvert f(x)\rvert = \max(f(x), 0) + \min(f(x), 0)
    \]
\end{proof}


\end{document}













