%!LW recipe=latexmk
\documentclass[11pt,a4paper]{article}
\input\input{../macros.tex}
\title{Learning Notes}
\author{Yingjie Zhu}
\date{\today}


\begin{document}
\maketitle

\section{Theory of Real Variable Function}

\begin{exercise}
    let $A$ be a measurable set and we have $m^*(A \triangle B) = 0$, prove that $B$ is also measurable, and $m(B) = m(A)$
\end{exercise}

\begin{proof}
    since we have $A \triangle B = \left( A \setminus B \right) \cup \left( B \setminus A \right)$, so 
    $m^*(A \setminus B) = m^*(B \setminus A) = 0$, and both $A \setminus B$, $B \setminus A$ are measurable.

    then we have

    \[
        B = (A \setminus (A \setminus B)) \cup (B \setminus A)
    \]

    so $B$ is measurable
\end{proof}

\begin{exercise}
    let $B$ meets that, for any $\epsilon > 0$, exists a measurable set $A$, so that $m^*(A \triangle B) \le \epsilon$, prove that
    $B$ is measurable.
\end{exercise}


\begin{proof}
    since $A$ is measurable, and $m^*(A \triangle B) \le \epsilon$, and we have
    consider that:

    \begin{align*}
        B &\subseteq A \cup B \subseteq A \cup (B \setminus A) \\
        B^C & \subseteq A^C \cup B^C \subseteq A^C \cup (B^C \setminus A^C) \subseteq A^C \cup (A \setminus B) 
    \end{align*}

    \begin{align*}
        m^*(T \cap B) &\le m^*(T \cap (A \cup (B \setminus A))) \le m^*(T \cap A) + m^*(T \cap (B \setminus A)) \\
        & \le m^*(T \cap A) + \epsilon \\
        m^*(T \cap B^C) & \le m^*(T \cap A^C) + m^*(T \cap (A \setminus B) \\
        & \le m^*(T \cap A^C) + \epsilon \\
m^*(T \cap B) + m^*(T \cap B^C) & \le  m^*(T \cap A) +  m^*(T \cap A^C) + 2\epsilon \\
& \le m^*(T) + 2\epsilon
    \end{align*}


take $\epsilon \to 0$, then we have

\[
m^*(T \cap B) + m^*(T \cap B^C) = m^*(T)
\]

\end{proof}

\begin{exercise}
    let $E \subseteq \mathbb{R}$ and $0 < \alpha < m(E)$, then exists $A \subseteq E$ 
    such that $A$ is bounded and closed. and $m(A) = \alpha$
\end{exercise}

\begin{proof}
    let's assume $E$ is bounded, otherwise we can take bounded subset $E'$ of $E$, so that  $m(E') > \alpha$
\end{proof}

\end{document}











